Improve code quality through better unfolding of spiders & Cexp automation

ZX.v
@@ -21,54 +21,64 @@ Definition bra_ket_MN (bra: Matrix 1 2) (ket : Vector 2) {n m} : Matrix (2 ^ m) 
   (m ⨂ ket) × (n ⨂ bra).
 Transparent bra_ket_MN. 
 
-Definition Spider_Semantics_Impl (bra0 bra1 : Matrix 1 2) (ket0 ket1 : Vector 2) (α : R) {n m : nat} : Matrix (2 ^ m) (2 ^ n) :=
+Lemma WF_bra_ket_MN : forall n m bra ket, WF_Matrix bra -> WF_Matrix ket -> WF_Matrix (@bra_ket_MN bra ket n m).
+Proof.
+  intros.
+  unfold bra_ket_MN.
+  apply WF_mult; restore_dims; apply WF_kron_n; assumption.
+Qed.
+
+Definition Spider_semantics (bra0 bra1 : Matrix 1 2) (ket0 ket1 : Vector 2) (α : R) {n m : nat} : Matrix (2 ^ m) (2 ^ n) :=
   (bra_ket_MN bra0 ket0) .+ (Cexp α) .* (bra_ket_MN bra1 ket1). 
-Transparent Spider_Semantics_Impl.
+Transparent Spider_semantics.
+
+Lemma WF_Spider_semantics : forall n m bra0 bra1 ket0 ket1 α, 
+                                WF_Matrix bra0 -> WF_Matrix bra1 -> WF_Matrix ket0 -> WF_Matrix ket1 -> 
+                                WF_Matrix (@Spider_semantics bra0 bra1 ket0 ket1 α n m).
+Proof.
+  intros.
+  unfold Spider_semantics.
+  apply WF_plus; restore_dims; try apply WF_scale; apply WF_bra_ket_MN; assumption.
+Qed.
+
+Global Hint Resolve WF_Spider_semantics WF_bra_ket_MN : wf_db.
 
 Fixpoint ZX_semantics {nIn nOut} (zx : ZX nIn nOut) : 
   Matrix (2 ^ nOut) (2 ^nIn) := 
   match zx with
   | Empty => I 1
-  | X_Spider _ _ α => Spider_Semantics_Impl (hadamard × (ket 0))† (hadamard × (ket 1))† (hadamard × (ket 0)) (hadamard × (ket 1)) α
-  | Z_Spider _ _ α => Spider_Semantics_Impl (bra 0) (bra 1) (ket 0) (ket 1) α
+  | X_Spider _ _ α => Spider_semantics (hadamard × (ket 0))† (hadamard × (ket 1))† (hadamard × (ket 0)) (hadamard × (ket 1)) α
+  | Z_Spider _ _ α => Spider_semantics (bra 0) (bra 1) (ket 0) (ket 1) α
   | Cup => list2D_to_matrix [[C1;C0;C0;C1]]
   | Cap => list2D_to_matrix [[C1];[C0];[C0];[C1]]  
   | Stack zx0 zx1 => (ZX_semantics zx0) ⊗ (ZX_semantics zx1)
   | Compose zx0 zx1 => (ZX_semantics zx1) × (ZX_semantics zx0)
   end.
 
+Ltac unfold_spider := unfold Spider_semantics, bra_ket_MN; try (simpl; Msimpl).
+
 Theorem WF_ZX : forall nIn nOut (zx : ZX nIn nOut), WF_Matrix (ZX_semantics zx).
 Proof.
   intros.
-  induction zx; try (simpl; auto 10 with wf_db).
-  - unfold Spider_Semantics_Impl, bra_ket_MN; try apply WF_plus; try apply WF_scale; apply WF_mult; try restore_dims; try auto with wf_db.
-  - unfold Spider_Semantics_Impl, bra_ket_MN; try apply WF_plus; try apply WF_scale; apply WF_mult; try restore_dims; try auto with wf_db.
-  - apply WF_list2D_to_matrix.
-    + easy.
-    + intros.
-      simpl in H; repeat destruct H; try discriminate; try (subst; easy).
-  - apply WF_list2D_to_matrix.
-    + easy.
-    + intros.
-      simpl in H; destruct H; try discriminate; try (subst; easy).
+  induction zx; try (simpl; auto 10 with wf_db);
+    apply WF_list2D_to_matrix;
+    try easy; (* case list of length 4 *)
+    try intros; simpl in H; repeat destruct H; try discriminate; try (subst; easy). (* Case of 4 lists length 1 *)
 Qed.
 
 Global Hint Resolve WF_ZX : wf_db.
 
 Definition Wire : ZX 1 1 := Z_Spider _ _ 0.
 
-Lemma bra_ket_id : ket 0 × bra 0 .+ ket 1 × bra 1 = I 2.
-Proof. solve_matrix. Qed.
-
 Theorem wire_identity_semantics : ZX_semantics Wire = I 2.
 Proof.
   simpl.
-  unfold Spider_Semantics_Impl, bra_ket_MN.
-  rewrite Cexp_0.
+  unfold_spider.
+  autorewrite with Cexp_db.
   rewrite Mscale_1_l.
   unfold kron_n.
   repeat rewrite kron_1_l; try auto with wf_db.
-  apply bra_ket_id.
+  solve_matrix.
 Qed.
 
 Global Opaque Wire.
