Eigenstates.v
@@ -6,26 +6,24 @@ Local Open Scope ZX_scope.
 Theorem ket_plus_state : ZX_semantics (Z_Spider 0 1 0) = √ 2 .* hadamard × (ket 0).
 Proof.
   simpl.
-  unfold Spider_Semantics_Impl, bra_ket_MN.
-  rewrite Cexp_0.
+  unfold_spider.
+  autorewrite with Cexp_db.
   solve_matrix.
 Qed.
 
 Theorem ket_minus_state : ZX_semantics (Z_Spider 0 1 PI) = √ 2 .* hadamard × (ket 1).
 Proof.
   simpl.
-  unfold Spider_Semantics_Impl, bra_ket_MN.
-  rewrite Cexp_PI.
+  unfold_spider.
+  autorewrite with Cexp_db.
   solve_matrix.
 Qed.
 
 Theorem ket_0_state : ZX_semantics (X_Spider 0 1 0) = √ 2 .* (ket 0).
 Proof.
   simpl.
-  unfold Spider_Semantics_Impl, bra_ket_MN.
-  rewrite Cexp_0.
-  simpl.
-  Msimpl.
+  unfold_spider.
+  autorewrite with Cexp_db.
   solve_matrix.
   C_field_simplify; try reflexivity; try apply Csqrt2_neq_0.
 Qed.
@@ -33,10 +31,8 @@ Qed.
 Theorem ket_1_state : ZX_semantics (X_Spider 0 1 PI) = √ 2 .* (ket 1).
 Proof.
   simpl.
-  unfold Spider_Semantics_Impl, bra_ket_MN.
-  rewrite Cexp_PI.
-  simpl.
-  Msimpl.
+  unfold_spider.
+  autorewrite with Cexp_db.
   solve_matrix.
   C_field_simplify; try lca; try apply Csqrt2_neq_0.
 Qed.
@@ -44,24 +40,24 @@ Qed.
 Theorem bra_plus_state : ZX_semantics (Z_Spider 1 0 0) = √ 2 .* (hadamard × (ket 0))†.
 Proof.
   simpl.
-  unfold Spider_Semantics_Impl, bra_ket_MN.
-  rewrite Cexp_0.
+  unfold_spider.
+  autorewrite with Cexp_db.
   solve_matrix.
 Qed.
 
 Theorem bra_minus_state : ZX_semantics (Z_Spider 1 0 PI) = √ 2 .* (hadamard × (ket 1))†.
 Proof.
   simpl.
-  unfold Spider_Semantics_Impl, bra_ket_MN.
-  rewrite Cexp_PI.
+  unfold_spider.
+  autorewrite with Cexp_db.
   solve_matrix.
 Qed.
 
 Theorem bra_0_state : ZX_semantics (X_Spider 1 0 0) = √ 2 .* (bra 0).
 Proof.
   simpl.
-  unfold Spider_Semantics_Impl, bra_ket_MN.
-  rewrite Cexp_0.
+  unfold_spider.
+  autorewrite with Cexp_db.
   solve_matrix.
   C_field_simplify; try reflexivity; try apply Csqrt2_neq_0.
 Qed.
@@ -69,8 +65,8 @@ Qed.
 Theorem bra_1_state : ZX_semantics (X_Spider 1 0 PI) = √ 2 .* (bra 1).
 Proof.
   simpl.
-  unfold Spider_Semantics_Impl, bra_ket_MN.
-  rewrite Cexp_PI.
+  unfold_spider.
+  autorewrite with Cexp_db.
   solve_matrix.
   C_field_simplify; try lca; try apply Csqrt2_neq_0.
 Qed.
